\input{../preamble.tex}


\title{Notes on Linear Algebra}
\begin{document}
\maketitle

\chapter{Preliminaries}
\section{Vector Spaces}
\subsection{Bases}
\subsection{Generating (span)}
\subsection{Independent System}

\begin{definition}[Independent]
  The system $\left\{\vec{v_1},\vec{v_2},\vec{v_3},\dots,
  \vec{v_n}\right\}$ are 
  called ``Independent'' iff
  \[
    \lambda_1\vec{v_1}+\lambda2\vec{v_2}+\cdots+
    \lambda_n\vec{v_n}=\vec{0}
    \iff \lambda_i=0
  \]
\end{definition}
\begin{definition}[Dependent]
  The system $\left\{\vec{v_1},\vec{v_2},
  \vec{v_3},\dots,\vec{v_n}\right\}$ are 
  called ``Dependent'' iff there exits some 
  $\lambda_j\neq 0$ such that $j<n$ and 
  \[\sum_{i=1}^{n}\lambda_i\vec{v_i}=\vec{0}\]
\end{definition}
\begin{proposition}
  The system $\left\{v_1,v_2,v_3,\dots,v_n\right\}$ are 
  dependent iff there exits $j$ such that 
  $\vec{v_j}$ is the linear combination of the other vectors.
\end{proposition}
\begin{proof}
  There exits $j<n$ such that $\lambda_j\neq 0$ and 
  \begin{align*}
    &\sum_{i=1}^{n}\lambda_i\vec{v_i}=\vec{0}\\
    \implies\quad &\lambda_j\vec{v_j}+
    \sum_{i\neq j}\lambda_i\vec{v_i}=\vec{0}\\
    \implies\quad &
    \vec{v_j}=\sum_{i\neq j}\frac{-\lambda_i}{\lambda_j}\vec{v_i}
  \end{align*}
  And the converse is simple to prove.
\end{proof}
\begin{proposition}
  If the system $\left\{v_1,v_2,v_3,\dots,v_n\right\}$ are
  both 
\end{proposition}
\begin{proposition}
  Bases $\iff$ Generating + Independent
\end{proposition}




\section{Linear Transformation}









\end{document}
